progs/verif_incr.v
@@ -1,4 +1,5 @@
 Require Import VST.progs.conclib.
+Require Import VST.progs.ghost.
 Require Import VST.progs.incr.
 
 Instance CompSpecs : compspecs. make_compspecs prog. Defined.
@@ -12,47 +13,53 @@ Definition spawn_spec := DECLARE _spawn spawn_spec.
 Definition freelock2_spec := DECLARE _freelock2 (freelock2_spec _).
 Definition release2_spec := DECLARE _release2 release2_spec.
 
-Definition cptr_lock_inv ctr := EX z : Z, data_at Ews tuint (Vint (Int.repr z)) ctr.
+Definition cptr_lock_inv g1 g2 ctr := EX z : Z, data_at Ews tuint (Vint (Int.repr z)) ctr *
+  EX x : Z, EX y : Z, !!(z = x + y) && ghost_var gsh1 x g1 * ghost_var gsh1 y g2.
 
 Definition incr_spec :=
  DECLARE _incr
-  WITH ctr : val, sh : share, lock : val
+  WITH ctr : val, sh : share, lock : val, g1 : gname, g2 : gname, left : bool
   PRE [ ]
          PROP  (readable_share sh)
          LOCAL (gvar _ctr ctr; gvar _ctr_lock lock)
-         SEP   (lock_inv sh lock (cptr_lock_inv ctr))
+         SEP   (lock_inv sh lock (cptr_lock_inv g1 g2 ctr); ghost_var gsh2 0 (if left then g1 else g2))
   POST [ tvoid ]
          PROP ()
          LOCAL ()
-         SEP (lock_inv sh lock (cptr_lock_inv ctr)).
+         SEP (lock_inv sh lock (cptr_lock_inv g1 g2 ctr); ghost_var gsh2 1 (if left then g1 else g2)).
 
 Definition read_spec :=
  DECLARE _read
-  WITH ctr : val, sh : share, lock : val
+  WITH ctr : val, sh : share, lock : val, g1 : gname, g2 : gname, n1 : Z, n2 : Z
   PRE [ ]
          PROP  (readable_share sh)
          LOCAL (gvar _ctr ctr; gvar _ctr_lock lock)
-         SEP   (lock_inv sh lock (cptr_lock_inv ctr))
-  POST [ tuint ] EX z : Z,
+         SEP   (lock_inv sh lock (cptr_lock_inv g1 g2 ctr); ghost_var gsh2 n1 g1; ghost_var gsh2 n2 g2)
+  POST [ tuint ]
          PROP ()
-         LOCAL (temp ret_temp (Vint (Int.repr z)))
-         SEP (lock_inv sh lock (cptr_lock_inv ctr)).
+         LOCAL (temp ret_temp (Vint (Int.repr (n1 + n2))))
+         SEP (lock_inv sh lock (cptr_lock_inv g1 g2 ctr); ghost_var gsh2 n1 g1; ghost_var gsh2 n2 g2).
 
-Definition thread_lock_inv sh ctr lockc lockt := selflock (lock_inv sh lockc (cptr_lock_inv ctr)) sh lockt.
+Definition thread_lock_R sh g1 g2 ctr lockc :=
+  lock_inv sh lockc (cptr_lock_inv g1 g2 ctr) * ghost_var gsh2 1 g1.
+
+Definition thread_lock_inv sh g1 g2 ctr lockc lockt :=
+  selflock (thread_lock_R sh g1 g2 ctr lockc) sh lockt.
 
 Definition thread_func_spec :=
  DECLARE _thread_func
-  WITH y : val, x : val * share * val * val
+  WITH y : val, x : val * share * val * val * gname * gname
   PRE [ _args OF (tptr tvoid) ]
-         let '(ctr, sh, lock, lockt) := x in
+         let '(ctr, sh, lock, lockt, g1, g2) := x in
          PROP  ()
          LOCAL (temp _args y; gvar _ctr ctr; gvar _ctr_lock lock; gvar _thread_lock lockt)
-         SEP   ((!!readable_share sh && emp); lock_inv sh lock (cptr_lock_inv ctr);
-                lock_inv sh lockt (thread_lock_inv sh ctr lock lockt))
+         SEP   ((!!readable_share sh && emp); lock_inv sh lock (cptr_lock_inv g1 g2 ctr);
+                ghost_var gsh2 0 g1;
+                lock_inv sh lockt (thread_lock_inv sh g1 g2 ctr lock lockt))
   POST [ tptr tvoid ]
          PROP ()
          LOCAL ()
-         SEP (emp).
+         SEP ().
 
 Definition main_spec :=
  DECLARE _main
@@ -63,48 +70,83 @@ Definition main_spec :=
 Definition Gprog : funspecs :=   ltac:(with_library prog [acquire_spec; release_spec; release2_spec; makelock_spec;
   freelock_spec; freelock2_spec; spawn_spec; incr_spec; read_spec; thread_func_spec; main_spec]).
 
-Lemma ctr_inv_precise : forall p,
-  precise (cptr_lock_inv p).
+Lemma ctr_inv_precise : forall g1 g2 p,
+  precise (cptr_lock_inv g1 g2 p).
 Proof.
-  intro; eapply derives_precise, data_at__precise with (sh := Ews)(t := tuint); auto.
-  intros ? (? & H); apply data_at_data_at_ in H; eauto.
-Qed.
+Admitted.
 Hint Resolve ctr_inv_precise.
 
-Lemma ctr_inv_positive : forall ctr,
-  positive_mpred (cptr_lock_inv ctr).
+Lemma ctr_inv_positive : forall g1 g2 ctr,
+  positive_mpred (cptr_lock_inv g1 g2 ctr).
 Proof.
-  intro; apply ex_positive; auto.
+  intros; unfold cptr_lock_inv.
+  apply ex_positive; intro.
+  apply positive_sepcon1; auto.
 Qed.
 Hint Resolve ctr_inv_positive.
+
+Lemma thread_inv_precise : forall sh g1 g2 ctr lock lockt,
+  precise (thread_lock_inv sh g1 g2 ctr lock lockt).
+Proof.
+  intros; apply selflock_precise, precise_sepcon; auto.
+Admitted.
+Hint Resolve thread_inv_precise.
 
 Lemma body_incr: semax_body Vprog Gprog f_incr incr_spec.
 Proof.
   start_function.
   forward.
-  forward_call (lock, sh, cptr_lock_inv ctr).
+  forward_call (lock, sh, cptr_lock_inv g1 g2 ctr).
   unfold cptr_lock_inv at 2; simpl.
-  Intro z.
+  Intros z x y.
   forward.
   forward.
-  forward_call (lock, sh, cptr_lock_inv ctr).
+  (* It would be nice to have a version of replace_SEP for view shift. *)
+  gather_SEP 2 3 4.
+  match goal with |-semax _ (PROPx _ (LOCALx ?Q (SEPx (_ :: ?R)))) _ _ =>
+    apply (semax_pre_bupd (PROP () (LOCALx Q
+      (SEPx (!!((if left then x else y) = 0) && ghost_var Tsh 1 (if left then g1 else g2) ::
+             ghost_var gsh1 (if left then y else x) (if left then g2 else g1) :: R))))) end.
+  { go_lower.
+    rewrite !prop_true_andp by auto.
+    rewrite <- 3sepcon_assoc.
+    eapply derives_trans; [|apply bupd_frame_r]; cancel.
+    destruct left.
+    - erewrite sepcon_assoc, sepcon_comm, sepcon_assoc, ghost_var_share_join' by (try apply sepalg.join_comm; eauto).
+      Intros; rewrite prop_true_andp by auto; eapply derives_trans, bupd_frame_r; cancel.
+      apply ghost_var_update.
+    - erewrite sepcon_assoc, ghost_var_share_join'; eauto.
+      Intros; rewrite prop_true_andp by auto; eapply derives_trans, bupd_frame_r; cancel.
+      apply ghost_var_update. }
+  Intros; forward_call (lock, sh, cptr_lock_inv g1 g2 ctr).
   { lock_props.
-    unfold cptr_lock_inv; Exists (z + 1); entailer!. }
+    unfold cptr_lock_inv; Exists (z + 1).
+    erewrite <- ghost_var_share_join by eauto.
+    unfold Frame; instantiate (1 := [ghost_var gsh2 1 (if left then g1 else g2)]); simpl.
+    destruct left.
+    - Exists 1 y; entailer!.
+    - Exists x 1; entailer!. }
   forward.
 Qed.
 
 Lemma body_read : semax_body Vprog Gprog f_read read_spec.
 Proof.
   start_function.
-  forward_call (lock, sh, cptr_lock_inv ctr).
+  forward_call (lock, sh, cptr_lock_inv g1 g2 ctr).
   unfold cptr_lock_inv at 2; simpl.
-  Intro z.
+  Intros z x y.
   forward.
-  forward_call (lock, sh, cptr_lock_inv ctr).
+  assert_PROP (x = n1 /\ y = n2) as Heq.
+  { go_lower.
+    rewrite <- sepcon_assoc, sepcon_comm; apply sepcon_derives_prop.
+    rewrite <- sepcon_prop_prop; eapply derives_trans; [|apply sepcon_derives; apply ghost_var_inj].
+    rewrite !sepcon_assoc; apply sepcon_derives; [apply derives_refl|].
+    rewrite <- sepcon_assoc, (sepcon_comm (ghost_var gsh1 y g2)), sepcon_assoc; apply derives_refl.
+    all: auto. }
+  forward_call (lock, sh, cptr_lock_inv g1 g2 ctr).
   { lock_props.
-    unfold cptr_lock_inv; Exists z; entailer!. }
-  forward.
-  Exists z; entailer!.
+    unfold cptr_lock_inv; Exists z x y; entailer!. }
+  destruct Heq; forward.
 Qed.
 
 Lemma body_thread_func : semax_body Vprog Gprog f_thread_func thread_func_spec.
@@ -112,10 +154,11 @@ Proof.
   start_function.
   Intros.
   forward.
-  forward_call (ctr, sh, lock).
-  forward_call (lockt, sh, lock_inv sh lock (cptr_lock_inv ctr), thread_lock_inv sh ctr lock lockt).
+  forward_call (ctr, sh, lock, g1, g2, true).
+  forward_call (lockt, sh, thread_lock_R sh g1 g2 ctr lock, thread_lock_inv sh g1 g2 ctr lock lockt).
   { unfold thread_lock_inv; lock_props.
-    rewrite selflock_eq at 2; cancel.
+    { apply thread_inv_precise. }
+    rewrite selflock_eq at 2; unfold thread_lock_R; cancel.
     eapply derives_trans; [apply lock_inv_later | cancel]. }
   forward.
 Qed.
@@ -129,30 +172,49 @@ Proof.
   (* temporarily broken *)
 Admitted.
 
+Lemma thread_ghost : forall sh g1 g2 ctr lock lockt,
+  thread_lock_inv sh g1 g2 ctr lock lockt =
+  ghost_var gsh2 1 g1 * (ghost_var gsh2 1 g1 -* thread_lock_inv sh g1 g2 ctr lock lockt).
+Proof.
+  intros; eapply wand_eq.
+  unfold thread_lock_inv, thread_lock_R.
+  rewrite selflock_eq.
+  rewrite (sepcon_comm _ (ghost_var _ _ _)), sepcon_assoc; eauto.
+Qed.
+
 Lemma body_main:  semax_body Vprog Gprog f_main main_spec.
 Proof.
   name ctr _ctr; name lockt _thread_lock; name lock _ctr_lock.
   start_function.
+  (* How should we get the initial inG's? *)
+  match goal with |-semax _ (PROPx ?P (LOCALx ?Q (SEPx ?R))) _ _ =>
+    apply (semax_pre (PROPx P (LOCALx Q (SEPx (inG (@pos_PCM (discrete_PCM Z)) :: R))))); [admit|] end.
   forward.
   forward.
   forward.
-  forward_call (lock, Ews, cptr_lock_inv ctr).
+  ghost_alloc (ghost_var Tsh 0).
+  Intro g1.
+  ghost_alloc (ghost_var Tsh 0).
+  Intro g2.
+  forward_call (lock, Ews, cptr_lock_inv g1 g2 ctr).
   { rewrite (sepcon_comm _ (fold_right_sepcon _)); apply sepcon_derives; [cancel | apply lock_struct]. }
-  forward_call (lock, Ews, cptr_lock_inv ctr).
+  forward_call (lock, Ews, cptr_lock_inv g1 g2 ctr).
   { lock_props.
-    unfold cptr_lock_inv; Exists 0; cancel. }
+    rewrite <- !(ghost_var_share_join gsh1 gsh2 Tsh) by auto.
+    unfold cptr_lock_inv; Exists 0 0 0; entailer!. }
   (* need to split off shares for the locks here *)
   destruct split_Ews as (sh1 & sh2 & ? & ? & Hsh).
-  forward_call (lockt, Ews, thread_lock_inv sh1 ctr lock lockt).
+  forward_call (lockt, Ews, thread_lock_inv sh1 g1 g2 ctr lock lockt).
   { rewrite (sepcon_comm _ (fold_right_sepcon _)); apply sepcon_derives; [cancel | apply lock_struct]. }
   get_global_function'' _thread_func.
   apply extract_exists_pre; intros f_.
-  forward_spawn (val * share * val * val)%type (f_, Vint (Int.repr 0),
-    fun x : val * share * val * val => let '(ctr, sh, lock, lockt) := x in
-      [(_ctr, ctr); (_ctr_lock, lock); (_thread_lock, lockt)], (ctr, sh1, lock, lockt),
-    fun (x : (val * share * val * val)) (_ : val) => let '(ctr, sh, lock, lockt) := x in
-         !!readable_share sh && emp * lock_inv sh lock (cptr_lock_inv ctr) *
-         lock_inv sh lockt (thread_lock_inv sh ctr lock lockt)).
+  forward_spawn (val * share * val * val * gname * gname)%type (f_, Vint (Int.repr 0),
+    fun x : val * share * val * val * gname * gname => let '(ctr, sh, lock, lockt, g1, g2) := x in
+      [(_ctr, ctr); (_ctr_lock, lock); (_thread_lock, lockt)], (ctr, sh1, lock, lockt, g1, g2),
+    fun (x : (val * share * val * val * gname * gname)) (_ : val) => let '(ctr, sh, lock, lockt, g1, g2) := x in
+         !!readable_share sh && emp * lock_inv sh lock (cptr_lock_inv g1 g2 ctr) *
+         ghost_var gsh2 0 g1 *
+         lock_inv sh lockt (thread_lock_inv sh g1 g2 ctr lock lockt)).
   { simpl spawn_pre; entailer!.
     { erewrite gvar_eval_var, !(force_val_sem_cast_neutral_gvar' _ f_) by eauto.
       split; auto; repeat split; apply gvar_denote_global; auto. }
@@ -165,27 +227,30 @@ Proof.
     erewrite <- lock_inv_share_join; try apply Hsh; auto.
     erewrite <- (lock_inv_share_join _ _ Ews); try apply Hsh; auto.
     entailer!. }
-  forward_call (ctr, sh2, lock).
-  forward_call (lockt, sh2, thread_lock_inv sh1 ctr lock lockt).
-  forward_call (ctr, sh2, lock).
-  Intro z.
-  forward_call (lock, sh2, cptr_lock_inv ctr).
-  forward_call (lockt, Ews, sh1, |>lock_inv sh1 lock (cptr_lock_inv ctr), |>thread_lock_inv sh1 ctr lock lockt).
+  forward_call (ctr, sh2, lock, g1, g2, false).
+  forward_call (lockt, sh2, thread_lock_inv sh1 g1 g2 ctr lock lockt).
+  rewrite thread_ghost at 2.
+  forward_call (ctr, sh2, lock, g1, g2, 1, 1).
+  gather_SEP 1 4; rewrite <- thread_ghost.
+  (* We've proved that t is 2! *)
+  forward_call (lock, sh2, cptr_lock_inv g1 g2 ctr).
+  forward_call (lockt, Ews, sh1, |>thread_lock_R sh1 g1 g2 ctr lock, |>thread_lock_inv sh1 g1 g2 ctr lock lockt).
   { unfold thread_lock_inv; lock_props.
     - apply later_positive; auto.
     - unfold rec_inv.
       rewrite selflock_eq at 1.
       rewrite later_sepcon; f_equal.
       apply lock_inv_later_eq.
-    - rewrite selflock_eq at 2.
+    - rewrite selflock_eq at 1.
       erewrite <- (lock_inv_share_join _ _ Ews); try apply Hsh; auto; cancel.
       rewrite sepcon_comm, <- !sepcon_assoc, sepcon_comm.
       apply sepcon_derives; [apply lock_inv_later | cancel]. }
-  forward_call (lock, Ews, cptr_lock_inv ctr).
+  forward_call (lock, Ews, cptr_lock_inv g1 g2 ctr).
   { lock_props.
-    erewrite sepcon_assoc, lock_inv_share_join; eauto; cancel. }
+    unfold thread_lock_R.
+    erewrite <- (lock_inv_share_join _ _ Ews); try apply Hsh; auto; cancel. }
   forward.
-Qed.
+Admitted.
 
 Definition extlink := ext_link_prog prog.
 
